fix: int -> uint; add sll_2_sllbseg, sll_2_sllb lemmas

TheoryTask/qcp-binary-democases/QCP_examples/sll_lib.c
@@ -104,7 +104,8 @@ struct sllb * cons_list_box(unsigned int data, struct sllb * box)
 {
     /*@ sllb(box, l)
         which implies
-        exists h pt, box -> head == h && box -> ptail == pt && sll(h, l)
+        exists h pt,
+            box -> head == h && box -> ptail == pt && sll(h, l)
     */
     box -> head = cons_list(data, box -> head);
     if (box -> ptail == & box -> head)
@@ -156,8 +157,10 @@ struct sllb * app_list_box(struct sllb * b1, struct sllb * b2)
     /*@ sllb(b1, l1) * sllb(b2, l2)
         which implies
         exists h1 pt1 h2 pt2,
-            b1 -> head == h1 && b1 -> ptail == pt1 && sllbseg(&(b1 -> head), pt1, l1) * store(pt1, struct sll *, 0) &&
-            b2 -> head == h2 && b2 -> ptail == pt2 && sll(h2, l2)
+            b1 -> head == h1 && b1 -> ptail == pt1 && 
+            b2 -> head == h2 && b2 -> ptail == pt2 &&
+            sllbseg(&(b1 -> head), pt1, l1) * store(pt1, struct sll *, 0) *
+            sllbseg(&(b2 -> head), pt2, l2) * store(pt2, struct sll *, 0)
     */
     * (b1 -> ptail) = b2 -> head;
     if (b2 -> head != (struct sll *) 0)
