TheoryTask/qcp-binary-democases/SeparationLogic/examples/sll_project_goal.v
@@ -441,37 +441,40 @@ forall (b2_pre: Z) (b1_pre: Z) (l2: (@list Z)) (l1: (@list Z)) (pt2: Z) (h2: Z) 
   ((( &( "b1" ) )) # Ptr  |-> b1_pre)
   **  ((&((b1_pre)  # "sllb" ->ₛ "head")) # Ptr  |-> h1)
   **  ((&((b1_pre)  # "sllb" ->ₛ "ptail")) # Ptr  |-> pt1)
-  **  (sllbseg &((b1_pre)  # "sllb" ->ₛ "head") pt1 l1 )
-  **  ((pt1) # Ptr  |-> h2)
   **  ((( &( "b2" ) )) # Ptr  |-> b2_pre)
   **  ((&((b2_pre)  # "sllb" ->ₛ "head")) # Ptr  |-> h2)
   **  ((&((b2_pre)  # "sllb" ->ₛ "ptail")) # Ptr  |-> pt2)
-  **  (sll h2 l2 )
+  **  (sllbseg &((b1_pre)  # "sllb" ->ₛ "head") pt1 l1 )
+  **  ((pt1) # Ptr  |-> h2)
+  **  (sllbseg &((b2_pre)  # "sllb" ->ₛ "head") pt2 l2 )
+  **  ((pt2) # Ptr  |-> 0)
 |--
   [| (0 <= INT_MAX) |] 
   &&  [| ((INT_MIN) <= 0) |]
 .
 
 Definition app_list_box_return_wit_1 := 
-forall (b1_pre: Z) (l2: (@list Z)) (l1: (@list Z)) (h2: Z) (pt1: Z) (h1: Z) ,
+forall (b2_pre: Z) (b1_pre: Z) (l2: (@list Z)) (l1: (@list Z)) (pt2: Z) (h2: Z) (pt1: Z) (h1: Z) ,
   [| (h2 = 0) |]
   &&  ((&((b1_pre)  # "sllb" ->ₛ "head")) # Ptr  |-> h1)
   **  ((&((b1_pre)  # "sllb" ->ₛ "ptail")) # Ptr  |-> pt1)
   **  (sllbseg &((b1_pre)  # "sllb" ->ₛ "head") pt1 l1 )
   **  ((pt1) # Ptr  |-> h2)
-  **  (sll h2 l2 )
+  **  (sllbseg &((b2_pre)  # "sllb" ->ₛ "head") pt2 l2 )
+  **  ((pt2) # Ptr  |-> 0)
 |--
   (sllb b1_pre (app (l1) (l2)) )
 .
 
 Definition app_list_box_return_wit_2 := 
-forall (b1_pre: Z) (l2: (@list Z)) (l1: (@list Z)) (pt2: Z) (h2: Z) (pt1: Z) (h1: Z) ,
+forall (b2_pre: Z) (b1_pre: Z) (l2: (@list Z)) (l1: (@list Z)) (pt2: Z) (h2: Z) (pt1: Z) (h1: Z) ,
   [| (h2 <> 0) |]
   &&  ((&((b1_pre)  # "sllb" ->ₛ "head")) # Ptr  |-> h1)
   **  ((&((b1_pre)  # "sllb" ->ₛ "ptail")) # Ptr  |-> pt2)
   **  (sllbseg &((b1_pre)  # "sllb" ->ₛ "head") pt1 l1 )
   **  ((pt1) # Ptr  |-> h2)
-  **  (sll h2 l2 )
+  **  (sllbseg &((b2_pre)  # "sllb" ->ₛ "head") pt2 l2 )
+  **  ((pt2) # Ptr  |-> 0)
 |--
   (sllb b1_pre (app (l1) (l2)) )
 .
@@ -490,11 +493,12 @@ forall (b2_pre: Z) (b1_pre: Z) (l2: (@list Z)) (l1: (@list Z)) (pt2: Z) (h2: Z) 
   [| (h2 <> 0) |]
   &&  ((&((b1_pre)  # "sllb" ->ₛ "head")) # Ptr  |-> h1)
   **  ((&((b1_pre)  # "sllb" ->ₛ "ptail")) # Ptr  |-> pt2)
-  **  (sllbseg &((b1_pre)  # "sllb" ->ₛ "head") pt1 l1 )
-  **  ((pt1) # Ptr  |-> h2)
   **  ((&((b2_pre)  # "sllb" ->ₛ "head")) # Ptr  |-> h2)
   **  ((&((b2_pre)  # "sllb" ->ₛ "ptail")) # Ptr  |-> pt2)
-  **  (sll h2 l2 )
+  **  (sllbseg &((b1_pre)  # "sllb" ->ₛ "head") pt1 l1 )
+  **  ((pt1) # Ptr  |-> h2)
+  **  (sllbseg &((b2_pre)  # "sllb" ->ₛ "head") pt2 l2 )
+  **  ((pt2) # Ptr  |-> 0)
 |--
   [| (h2 <> 0) |]
   &&  ((&((b2_pre)  # "sllb" ->ₛ "head")) # Ptr  |-> h2)
@@ -503,7 +507,8 @@ forall (b2_pre: Z) (b1_pre: Z) (l2: (@list Z)) (l1: (@list Z)) (pt2: Z) (h2: Z) 
   **  ((&((b1_pre)  # "sllb" ->ₛ "ptail")) # Ptr  |-> pt2)
   **  (sllbseg &((b1_pre)  # "sllb" ->ₛ "head") pt1 l1 )
   **  ((pt1) # Ptr  |-> h2)
-  **  (sll h2 l2 )
+  **  (sllbseg &((b2_pre)  # "sllb" ->ₛ "head") pt2 l2 )
+  **  ((pt2) # Ptr  |-> 0)
 .
 
 Definition app_list_box_partial_solve_wit_3 := 
@@ -511,11 +516,12 @@ forall (b2_pre: Z) (b1_pre: Z) (l2: (@list Z)) (l1: (@list Z)) (pt2: Z) (h2: Z) 
   [| (h2 = 0) |]
   &&  ((&((b1_pre)  # "sllb" ->ₛ "head")) # Ptr  |-> h1)
   **  ((&((b1_pre)  # "sllb" ->ₛ "ptail")) # Ptr  |-> pt1)
-  **  (sllbseg &((b1_pre)  # "sllb" ->ₛ "head") pt1 l1 )
-  **  ((pt1) # Ptr  |-> h2)
   **  ((&((b2_pre)  # "sllb" ->ₛ "head")) # Ptr  |-> h2)
   **  ((&((b2_pre)  # "sllb" ->ₛ "ptail")) # Ptr  |-> pt2)
-  **  (sll h2 l2 )
+  **  (sllbseg &((b1_pre)  # "sllb" ->ₛ "head") pt1 l1 )
+  **  ((pt1) # Ptr  |-> h2)
+  **  (sllbseg &((b2_pre)  # "sllb" ->ₛ "head") pt2 l2 )
+  **  ((pt2) # Ptr  |-> 0)
 |--
   [| (h2 = 0) |]
   &&  ((&((b2_pre)  # "sllb" ->ₛ "head")) # Ptr  |-> h2)
@@ -524,7 +530,8 @@ forall (b2_pre: Z) (b1_pre: Z) (l2: (@list Z)) (l1: (@list Z)) (pt2: Z) (h2: Z) 
   **  ((&((b1_pre)  # "sllb" ->ₛ "ptail")) # Ptr  |-> pt1)
   **  (sllbseg &((b1_pre)  # "sllb" ->ₛ "head") pt1 l1 )
   **  ((pt1) # Ptr  |-> h2)
-  **  (sll h2 l2 )
+  **  (sllbseg &((b2_pre)  # "sllb" ->ₛ "head") pt2 l2 )
+  **  ((pt2) # Ptr  |-> 0)
 .
 
 Definition app_list_box_which_implies_wit_1 := 
@@ -535,11 +542,12 @@ forall (l2: (@list Z)) (l1: (@list Z)) (b1: Z) (b2: Z) ,
   EX (pt2: Z)  (h2: Z)  (pt1: Z)  (h1: Z) ,
   ((&((b1)  # "sllb" ->ₛ "head")) # Ptr  |-> h1)
   **  ((&((b1)  # "sllb" ->ₛ "ptail")) # Ptr  |-> pt1)
-  **  (sllbseg &((b1)  # "sllb" ->ₛ "head") pt1 l1 )
-  **  ((pt1) # Ptr  |-> 0)
   **  ((&((b2)  # "sllb" ->ₛ "head")) # Ptr  |-> h2)
   **  ((&((b2)  # "sllb" ->ₛ "ptail")) # Ptr  |-> pt2)
-  **  (sll h2 l2 )
+  **  (sllbseg &((b1)  # "sllb" ->ₛ "head") pt1 l1 )
+  **  ((pt1) # Ptr  |-> 0)
+  **  (sllbseg &((b2)  # "sllb" ->ₛ "head") pt2 l2 )
+  **  ((pt2) # Ptr  |-> 0)
 .
 
 (*----- Function sll_length -----*)
